fstar

libcrux-ml-dsa/proofs/fstar/extraction/Libcrux_ml_dsa.Hash_functions.Portable.fsti
@@ -21,6 +21,18 @@ val t_Shake256Absorb:Type0
 
 val t_Shake256Squeeze:Type0
 
+[@@ FStar.Tactics.Typeclasses.tcinstance]
+val impl:Libcrux_ml_dsa.Hash_functions.Shake128.t_XofX4 t_Shake128X4
+
+[@@ FStar.Tactics.Typeclasses.tcinstance]
+val impl_1:Libcrux_ml_dsa.Hash_functions.Shake128.t_Xof t_Shake128
+
+[@@ FStar.Tactics.Typeclasses.tcinstance]
+val impl_2:Libcrux_ml_dsa.Hash_functions.Shake256.t_Xof t_Shake256
+
+[@@ FStar.Tactics.Typeclasses.tcinstance]
+val impl_3:Libcrux_ml_dsa.Hash_functions.Shake256.t_XofX4 t_Shake256X4
+
 val init_absorb (input0 input1 input2 input3: t_Slice u8)
     : Prims.Pure t_Shake128X4 Prims.l_True (fun _ -> Prims.l_True)
 
@@ -32,28 +44,6 @@ val init_absorb_x4 (input0 input1 input2 input3: t_Slice u8)
 
 val shake128 (v_OUTPUT_LENGTH: usize) (input: t_Slice u8) (out: t_Array u8 v_OUTPUT_LENGTH)
     : Prims.Pure (t_Array u8 v_OUTPUT_LENGTH) Prims.l_True (fun _ -> Prims.l_True)
-
-[@@ FStar.Tactics.Typeclasses.tcinstance]
-let impl_1: Libcrux_ml_dsa.Hash_functions.Shake128.t_Xof t_Shake128 =
-  {
-    f_shake128_pre
-    =
-    (fun (v_OUTPUT_LENGTH: usize) (input: t_Slice u8) (out: t_Array u8 v_OUTPUT_LENGTH) -> true);
-    f_shake128_post
-    =
-    (fun
-        (v_OUTPUT_LENGTH: usize)
-        (input: t_Slice u8)
-        (out: t_Array u8 v_OUTPUT_LENGTH)
-        (out1: t_Array u8 v_OUTPUT_LENGTH)
-        ->
-        true);
-    f_shake128
-    =
-    fun (v_OUTPUT_LENGTH: usize) (input: t_Slice u8) (out: t_Array u8 v_OUTPUT_LENGTH) ->
-      let out:t_Array u8 v_OUTPUT_LENGTH = shake128 v_OUTPUT_LENGTH input out in
-      out
-  }
 
 val shake256 (v_OUTPUT_LENGTH: usize) (input: t_Slice u8) (out: t_Array u8 v_OUTPUT_LENGTH)
     : Prims.Pure (t_Array u8 v_OUTPUT_LENGTH) Prims.l_True (fun _ -> Prims.l_True)
@@ -91,152 +81,8 @@ val squeeze_next_block (state: t_Shake128X4)
       Prims.l_True
       (fun _ -> Prims.l_True)
 
-[@@ FStar.Tactics.Typeclasses.tcinstance]
-let impl: Libcrux_ml_dsa.Hash_functions.Shake128.t_XofX4 t_Shake128X4 =
-  {
-    f_init_absorb_pre
-    =
-    (fun (input0: t_Slice u8) (input1: t_Slice u8) (input2: t_Slice u8) (input3: t_Slice u8) -> true
-    );
-    f_init_absorb_post
-    =
-    (fun
-        (input0: t_Slice u8)
-        (input1: t_Slice u8)
-        (input2: t_Slice u8)
-        (input3: t_Slice u8)
-        (out: t_Shake128X4)
-        ->
-        true);
-    f_init_absorb
-    =
-    (fun (input0: t_Slice u8) (input1: t_Slice u8) (input2: t_Slice u8) (input3: t_Slice u8) ->
-        init_absorb input0 input1 input2 input3);
-    f_squeeze_first_five_blocks_pre
-    =
-    (fun
-        (self: t_Shake128X4)
-        (out0: t_Array u8 (sz 840))
-        (out1: t_Array u8 (sz 840))
-        (out2: t_Array u8 (sz 840))
-        (out3: t_Array u8 (sz 840))
-        ->
-        true);
-    f_squeeze_first_five_blocks_post
-    =
-    (fun
-        (self: t_Shake128X4)
-        (out0: t_Array u8 (sz 840))
-        (out1: t_Array u8 (sz 840))
-        (out2: t_Array u8 (sz 840))
-        (out3: t_Array u8 (sz 840))
-        (out4:
-          (t_Shake128X4 & t_Array u8 (sz 840) & t_Array u8 (sz 840) & t_Array u8 (sz 840) &
-            t_Array u8 (sz 840)))
-        ->
-        true);
-    f_squeeze_first_five_blocks
-    =
-    (fun
-        (self: t_Shake128X4)
-        (out0: t_Array u8 (sz 840))
-        (out1: t_Array u8 (sz 840))
-        (out2: t_Array u8 (sz 840))
-        (out3: t_Array u8 (sz 840))
-        ->
-        let tmp0, tmp1, tmp2, tmp3, tmp4:(t_Shake128X4 & t_Array u8 (sz 840) & t_Array u8 (sz 840) &
-          t_Array u8 (sz 840) &
-          t_Array u8 (sz 840)) =
-          squeeze_first_five_blocks self out0 out1 out2 out3
-        in
-        let self:t_Shake128X4 = tmp0 in
-        let out0:t_Array u8 (sz 840) = tmp1 in
-        let out1:t_Array u8 (sz 840) = tmp2 in
-        let out2:t_Array u8 (sz 840) = tmp3 in
-        let out3:t_Array u8 (sz 840) = tmp4 in
-        let _:Prims.unit = () in
-        self, out0, out1, out2, out3
-        <:
-        (t_Shake128X4 & t_Array u8 (sz 840) & t_Array u8 (sz 840) & t_Array u8 (sz 840) &
-          t_Array u8 (sz 840)));
-    f_squeeze_next_block_pre = (fun (self: t_Shake128X4) -> true);
-    f_squeeze_next_block_post
-    =
-    (fun
-        (self: t_Shake128X4)
-        (out5:
-          (t_Shake128X4 &
-            (t_Array u8 (sz 168) & t_Array u8 (sz 168) & t_Array u8 (sz 168) & t_Array u8 (sz 168)))
-        )
-        ->
-        true);
-    f_squeeze_next_block
-    =
-    fun (self: t_Shake128X4) ->
-      let tmp0, out4:(t_Shake128X4 &
-        (t_Array u8 (sz 168) & t_Array u8 (sz 168) & t_Array u8 (sz 168) & t_Array u8 (sz 168))) =
-        squeeze_next_block self
-      in
-      let self:t_Shake128X4 = tmp0 in
-      let hax_temp_output:(t_Array u8 (sz 168) & t_Array u8 (sz 168) & t_Array u8 (sz 168) &
-        t_Array u8 (sz 168)) =
-        out4
-      in
-      self, hax_temp_output
-      <:
-      (t_Shake128X4 &
-        (t_Array u8 (sz 168) & t_Array u8 (sz 168) & t_Array u8 (sz 168) & t_Array u8 (sz 168)))
-  }
-
 val squeeze_next_block_shake256 (state: t_Shake256)
     : Prims.Pure (t_Shake256 & t_Array u8 (sz 136)) Prims.l_True (fun _ -> Prims.l_True)
-
-[@@ FStar.Tactics.Typeclasses.tcinstance]
-let impl_2: Libcrux_ml_dsa.Hash_functions.Shake256.t_Xof t_Shake256 =
-  {
-    f_shake256_pre
-    =
-    (fun (v_OUTPUT_LENGTH: usize) (input: t_Slice u8) (out: t_Array u8 v_OUTPUT_LENGTH) -> true);
-    f_shake256_post
-    =
-    (fun
-        (v_OUTPUT_LENGTH: usize)
-        (input: t_Slice u8)
-        (out: t_Array u8 v_OUTPUT_LENGTH)
-        (out1: t_Array u8 v_OUTPUT_LENGTH)
-        ->
-        true);
-    f_shake256
-    =
-    (fun (v_OUTPUT_LENGTH: usize) (input: t_Slice u8) (out: t_Array u8 v_OUTPUT_LENGTH) ->
-        let out:t_Array u8 v_OUTPUT_LENGTH = shake256 v_OUTPUT_LENGTH input out in
-        out);
-    f_init_absorb_pre = (fun (input: t_Slice u8) -> true);
-    f_init_absorb_post = (fun (input: t_Slice u8) (out: t_Shake256) -> true);
-    f_init_absorb = (fun (input: t_Slice u8) -> init_absorb_shake256 input);
-    f_squeeze_first_block_pre = (fun (self: t_Shake256) -> true);
-    f_squeeze_first_block_post
-    =
-    (fun (self: t_Shake256) (out2: (t_Shake256 & t_Array u8 (sz 136))) -> true);
-    f_squeeze_first_block
-    =
-    (fun (self: t_Shake256) ->
-        let tmp0, out1:(t_Shake256 & t_Array u8 (sz 136)) = squeeze_first_block_shake256 self in
-        let self:t_Shake256 = tmp0 in
-        let hax_temp_output:t_Array u8 (sz 136) = out1 in
-        self, hax_temp_output <: (t_Shake256 & t_Array u8 (sz 136)));
-    f_squeeze_next_block_pre = (fun (self: t_Shake256) -> true);
-    f_squeeze_next_block_post
-    =
-    (fun (self: t_Shake256) (out2: (t_Shake256 & t_Array u8 (sz 136))) -> true);
-    f_squeeze_next_block
-    =
-    fun (self: t_Shake256) ->
-      let tmp0, out1:(t_Shake256 & t_Array u8 (sz 136)) = squeeze_next_block_shake256 self in
-      let self:t_Shake256 = tmp0 in
-      let hax_temp_output:t_Array u8 (sz 136) = out1 in
-      self, hax_temp_output <: (t_Shake256 & t_Array u8 (sz 136))
-  }
 
 val squeeze_next_block_x4 (state: t_Shake256X4)
     : Prims.Pure
@@ -244,131 +90,3 @@ val squeeze_next_block_x4 (state: t_Shake256X4)
         (t_Array u8 (sz 136) & t_Array u8 (sz 136) & t_Array u8 (sz 136) & t_Array u8 (sz 136)))
       Prims.l_True
       (fun _ -> Prims.l_True)
-
-[@@ FStar.Tactics.Typeclasses.tcinstance]
-let impl_3: Libcrux_ml_dsa.Hash_functions.Shake256.t_XofX4 t_Shake256X4 =
-  {
-    f_init_absorb_x4_pre
-    =
-    (fun (input0: t_Slice u8) (input1: t_Slice u8) (input2: t_Slice u8) (input3: t_Slice u8) -> true
-    );
-    f_init_absorb_x4_post
-    =
-    (fun
-        (input0: t_Slice u8)
-        (input1: t_Slice u8)
-        (input2: t_Slice u8)
-        (input3: t_Slice u8)
-        (out: t_Shake256X4)
-        ->
-        true);
-    f_init_absorb_x4
-    =
-    (fun (input0: t_Slice u8) (input1: t_Slice u8) (input2: t_Slice u8) (input3: t_Slice u8) ->
-        init_absorb_x4 input0 input1 input2 input3);
-    f_squeeze_first_block_x4_pre = (fun (self: t_Shake256X4) -> true);
-    f_squeeze_first_block_x4_post
-    =
-    (fun
-        (self: t_Shake256X4)
-        (out5:
-          (t_Shake256X4 &
-            (t_Array u8 (sz 136) & t_Array u8 (sz 136) & t_Array u8 (sz 136) & t_Array u8 (sz 136)))
-        )
-        ->
-        true);
-    f_squeeze_first_block_x4
-    =
-    (fun (self: t_Shake256X4) ->
-        let tmp0, out4:(t_Shake256X4 &
-          (t_Array u8 (sz 136) & t_Array u8 (sz 136) & t_Array u8 (sz 136) & t_Array u8 (sz 136))) =
-          squeeze_first_block_x4 self
-        in
-        let self:t_Shake256X4 = tmp0 in
-        let hax_temp_output:(t_Array u8 (sz 136) & t_Array u8 (sz 136) & t_Array u8 (sz 136) &
-          t_Array u8 (sz 136)) =
-          out4
-        in
-        self, hax_temp_output
-        <:
-        (t_Shake256X4 &
-          (t_Array u8 (sz 136) & t_Array u8 (sz 136) & t_Array u8 (sz 136) & t_Array u8 (sz 136))));
-    f_squeeze_next_block_x4_pre = (fun (self: t_Shake256X4) -> true);
-    f_squeeze_next_block_x4_post
-    =
-    (fun
-        (self: t_Shake256X4)
-        (out5:
-          (t_Shake256X4 &
-            (t_Array u8 (sz 136) & t_Array u8 (sz 136) & t_Array u8 (sz 136) & t_Array u8 (sz 136)))
-        )
-        ->
-        true);
-    f_squeeze_next_block_x4
-    =
-    (fun (self: t_Shake256X4) ->
-        let tmp0, out4:(t_Shake256X4 &
-          (t_Array u8 (sz 136) & t_Array u8 (sz 136) & t_Array u8 (sz 136) & t_Array u8 (sz 136))) =
-          squeeze_next_block_x4 self
-        in
-        let self:t_Shake256X4 = tmp0 in
-        let hax_temp_output:(t_Array u8 (sz 136) & t_Array u8 (sz 136) & t_Array u8 (sz 136) &
-          t_Array u8 (sz 136)) =
-          out4
-        in
-        self, hax_temp_output
-        <:
-        (t_Shake256X4 &
-          (t_Array u8 (sz 136) & t_Array u8 (sz 136) & t_Array u8 (sz 136) & t_Array u8 (sz 136))));
-    f_shake256_x4_pre
-    =
-    (fun
-        (v_OUT_LEN: usize)
-        (input0: t_Slice u8)
-        (input1: t_Slice u8)
-        (input2: t_Slice u8)
-        (input3: t_Slice u8)
-        (out0: t_Array u8 v_OUT_LEN)
-        (out1: t_Array u8 v_OUT_LEN)
-        (out2: t_Array u8 v_OUT_LEN)
-        (out3: t_Array u8 v_OUT_LEN)
-        ->
-        true);
-    f_shake256_x4_post
-    =
-    (fun
-        (v_OUT_LEN: usize)
-        (input0: t_Slice u8)
-        (input1: t_Slice u8)
-        (input2: t_Slice u8)
-        (input3: t_Slice u8)
-        (out0: t_Array u8 v_OUT_LEN)
-        (out1: t_Array u8 v_OUT_LEN)
-        (out2: t_Array u8 v_OUT_LEN)
-        (out3: t_Array u8 v_OUT_LEN)
-        (out4:
-          (t_Array u8 v_OUT_LEN & t_Array u8 v_OUT_LEN & t_Array u8 v_OUT_LEN & t_Array u8 v_OUT_LEN
-          ))
-        ->
-        true);
-    f_shake256_x4
-    =
-    fun
-      (v_OUT_LEN: usize)
-      (input0: t_Slice u8)
-      (input1: t_Slice u8)
-      (input2: t_Slice u8)
-      (input3: t_Slice u8)
-      (out0: t_Array u8 v_OUT_LEN)
-      (out1: t_Array u8 v_OUT_LEN)
-      (out2: t_Array u8 v_OUT_LEN)
-      (out3: t_Array u8 v_OUT_LEN)
-      ->
-      let out0:t_Array u8 v_OUT_LEN = shake256 v_OUT_LEN input0 out0 in
-      let out1:t_Array u8 v_OUT_LEN = shake256 v_OUT_LEN input1 out1 in
-      let out2:t_Array u8 v_OUT_LEN = shake256 v_OUT_LEN input2 out2 in
-      let out3:t_Array u8 v_OUT_LEN = shake256 v_OUT_LEN input3 out3 in
-      out0, out1, out2, out3
-      <:
-      (t_Array u8 v_OUT_LEN & t_Array u8 v_OUT_LEN & t_Array u8 v_OUT_LEN & t_Array u8 v_OUT_LEN)
-  }
