libcrux-ml-dsa/proofs/fstar/extraction/Libcrux_ml_dsa.Simd.Avx2.Vector_type.fsti
@@ -6,17 +6,7 @@ open FStar.Mul
 type t_AVX2SIMDUnit = { f_coefficients:Libcrux_intrinsics.Avx2_extract.t_Vec256 }
 
 [@@ FStar.Tactics.Typeclasses.tcinstance]
-let impl: Core.Convert.t_From t_AVX2SIMDUnit Libcrux_intrinsics.Avx2_extract.t_Vec256 =
-  {
-    f_from_pre = (fun (coefficients: Libcrux_intrinsics.Avx2_extract.t_Vec256) -> true);
-    f_from_post
-    =
-    (fun (coefficients: Libcrux_intrinsics.Avx2_extract.t_Vec256) (out: t_AVX2SIMDUnit) -> true);
-    f_from
-    =
-    fun (coefficients: Libcrux_intrinsics.Avx2_extract.t_Vec256) ->
-      { f_coefficients = coefficients } <: t_AVX2SIMDUnit
-  }
+val impl:Core.Convert.t_From t_AVX2SIMDUnit Libcrux_intrinsics.Avx2_extract.t_Vec256
 
 val v_ZERO: Prims.unit -> Prims.Pure t_AVX2SIMDUnit Prims.l_True (fun _ -> Prims.l_True)
 
