libcrux-ml-kem/proofs/fstar/extraction/Libcrux_ml_kem.Hash_functions.Avx2.fsti
@@ -8,6 +8,9 @@ open FStar.Mul
 /// All other functions don\'t actually use any members.
 val t_Simd256Hash:Type0
 
+[@@ FStar.Tactics.Typeclasses.tcinstance]
+val impl (v_K: usize) : Libcrux_ml_kem.Hash_functions.t_Hash t_Simd256Hash v_K
+
 val v_G (input: t_Slice u8)
     : Prims.Pure (t_Array u8 (sz 64))
       Prims.l_True
@@ -52,69 +55,3 @@ val shake128_squeeze_next_block (v_K: usize) (st: t_Simd256Hash)
     : Prims.Pure (t_Simd256Hash & t_Array (t_Array u8 (sz 168)) v_K)
       Prims.l_True
       (fun _ -> Prims.l_True)
-
-[@@ FStar.Tactics.Typeclasses.tcinstance]
-let impl (v_K: usize) : Libcrux_ml_kem.Hash_functions.t_Hash t_Simd256Hash v_K =
-  {
-    f_G_pre = (fun (input: t_Slice u8) -> true);
-    f_G_post = (fun (input: t_Slice u8) (out: t_Array u8 (sz 64)) -> out == Spec.Utils.v_G input);
-    f_G = (fun (input: t_Slice u8) -> v_G input);
-    f_H_pre = (fun (input: t_Slice u8) -> true);
-    f_H_post = (fun (input: t_Slice u8) (out: t_Array u8 (sz 32)) -> out == Spec.Utils.v_H input);
-    f_H = (fun (input: t_Slice u8) -> v_H input);
-    f_PRF_pre = (fun (v_LEN: usize) (input: t_Slice u8) -> v v_LEN < pow2 32);
-    f_PRF_post
-    =
-    (fun (v_LEN: usize) (input: t_Slice u8) (out: t_Array u8 v_LEN) ->
-        v v_LEN < pow2 32 ==> out == Spec.Utils.v_PRF v_LEN input);
-    f_PRF = (fun (v_LEN: usize) (input: t_Slice u8) -> v_PRF v_LEN input);
-    f_PRFxN_pre
-    =
-    (fun (v_LEN: usize) (input: t_Array (t_Array u8 (sz 33)) v_K) ->
-        v v_LEN < pow2 32 /\ (v v_K == 2 \/ v v_K == 3 \/ v v_K == 4));
-    f_PRFxN_post
-    =
-    (fun
-        (v_LEN: usize)
-        (input: t_Array (t_Array u8 (sz 33)) v_K)
-        (out: t_Array (t_Array u8 v_LEN) v_K)
-        ->
-        (v v_LEN < pow2 32 /\ (v v_K == 2 \/ v v_K == 3 \/ v v_K == 4)) ==>
-        out == Spec.Utils.v_PRFxN v_K v_LEN input);
-    f_PRFxN
-    =
-    (fun (v_LEN: usize) (input: t_Array (t_Array u8 (sz 33)) v_K) -> v_PRFxN v_K v_LEN input);
-    f_shake128_init_absorb_final_pre = (fun (input: t_Array (t_Array u8 (sz 34)) v_K) -> true);
-    f_shake128_init_absorb_final_post
-    =
-    (fun (input: t_Array (t_Array u8 (sz 34)) v_K) (out: t_Simd256Hash) -> true);
-    f_shake128_init_absorb_final
-    =
-    (fun (input: t_Array (t_Array u8 (sz 34)) v_K) -> shake128_init_absorb_final v_K input);
-    f_shake128_squeeze_first_three_blocks_pre = (fun (self: t_Simd256Hash) -> true);
-    f_shake128_squeeze_first_three_blocks_post
-    =
-    (fun (self: t_Simd256Hash) (out1: (t_Simd256Hash & t_Array (t_Array u8 (sz 504)) v_K)) -> true);
-    f_shake128_squeeze_first_three_blocks
-    =
-    (fun (self: t_Simd256Hash) ->
-        let tmp0, out:(t_Simd256Hash & t_Array (t_Array u8 (sz 504)) v_K) =
-          shake128_squeeze_first_three_blocks v_K self
-        in
-        let self:t_Simd256Hash = tmp0 in
-        let hax_temp_output:t_Array (t_Array u8 (sz 504)) v_K = out in
-        self, hax_temp_output <: (t_Simd256Hash & t_Array (t_Array u8 (sz 504)) v_K));
-    f_shake128_squeeze_next_block_pre = (fun (self: t_Simd256Hash) -> true);
-    f_shake128_squeeze_next_block_post
-    =
-    (fun (self: t_Simd256Hash) (out1: (t_Simd256Hash & t_Array (t_Array u8 (sz 168)) v_K)) -> true);
-    f_shake128_squeeze_next_block
-    =
-    fun (self: t_Simd256Hash) ->
-      let tmp0, out:(t_Simd256Hash & t_Array (t_Array u8 (sz 168)) v_K) =
-        shake128_squeeze_next_block v_K self
-      in
-      let self:t_Simd256Hash = tmp0 in
-      let hax_temp_output:t_Array (t_Array u8 (sz 168)) v_K = out in
-      self, hax_temp_output <: (t_Simd256Hash & t_Array (t_Array u8 (sz 168)) v_K)
-  }
