libcrux-ml-kem/proofs/fstar/extraction/Libcrux_ml_kem.Ind_cpa.Unpacked.fsti
@@ -24,65 +24,15 @@ type t_IndCpaPublicKeyUnpacked
 }
 
 [@@ FStar.Tactics.Typeclasses.tcinstance]
-let impl
+val impl
       (v_K: usize)
       (#v_Vector: Type0)
-      (#[FStar.Tactics.Typeclasses.tcresolve ()]
-          i1:
-          Libcrux_ml_kem.Vector.Traits.t_Operations v_Vector)
-    : Core.Default.t_Default (t_IndCpaPrivateKeyUnpacked v_K v_Vector) =
-  {
-    f_default_pre = (fun (_: Prims.unit) -> true);
-    f_default_post = (fun (_: Prims.unit) (out: t_IndCpaPrivateKeyUnpacked v_K v_Vector) -> true);
-    f_default
-    =
-    fun (_: Prims.unit) ->
-      {
-        f_secret_as_ntt
-        =
-        Rust_primitives.Hax.repeat (Libcrux_ml_kem.Polynomial.impl_2__ZERO #v_Vector ()
-            <:
-            Libcrux_ml_kem.Polynomial.t_PolynomialRingElement v_Vector)
-          v_K
-      }
-      <:
-      t_IndCpaPrivateKeyUnpacked v_K v_Vector
-  }
+      {| i1: Libcrux_ml_kem.Vector.Traits.t_Operations v_Vector |}
+    : Core.Default.t_Default (t_IndCpaPrivateKeyUnpacked v_K v_Vector)
 
 [@@ FStar.Tactics.Typeclasses.tcinstance]
-let impl_1
+val impl_1
       (v_K: usize)
       (#v_Vector: Type0)
-      (#[FStar.Tactics.Typeclasses.tcresolve ()]
-          i1:
-          Libcrux_ml_kem.Vector.Traits.t_Operations v_Vector)
-    : Core.Default.t_Default (t_IndCpaPublicKeyUnpacked v_K v_Vector) =
-  {
-    f_default_pre = (fun (_: Prims.unit) -> true);
-    f_default_post = (fun (_: Prims.unit) (out: t_IndCpaPublicKeyUnpacked v_K v_Vector) -> true);
-    f_default
-    =
-    fun (_: Prims.unit) ->
-      {
-        f_t_as_ntt
-        =
-        Rust_primitives.Hax.repeat (Libcrux_ml_kem.Polynomial.impl_2__ZERO #v_Vector ()
-            <:
-            Libcrux_ml_kem.Polynomial.t_PolynomialRingElement v_Vector)
-          v_K;
-        f_seed_for_A = Rust_primitives.Hax.repeat 0uy (sz 32);
-        f_A
-        =
-        Rust_primitives.Hax.repeat (Rust_primitives.Hax.repeat (Libcrux_ml_kem.Polynomial.impl_2__ZERO
-                  #v_Vector
-                  ()
-                <:
-                Libcrux_ml_kem.Polynomial.t_PolynomialRingElement v_Vector)
-              v_K
-            <:
-            t_Array (Libcrux_ml_kem.Polynomial.t_PolynomialRingElement v_Vector) v_K)
-          v_K
-      }
-      <:
-      t_IndCpaPublicKeyUnpacked v_K v_Vector
-  }
+      {| i1: Libcrux_ml_kem.Vector.Traits.t_Operations v_Vector |}
+    : Core.Default.t_Default (t_IndCpaPublicKeyUnpacked v_K v_Vector)
