libcrux-ml-kem/proofs/fstar/extraction/Libcrux_ml_kem.Types.fsti
@@ -19,33 +19,13 @@ val impl_20__len: v_SIZE: usize -> Prims.unit
 type t_MlKemCiphertext (v_SIZE: usize) = { f_value:t_Array u8 v_SIZE }
 
 [@@ FStar.Tactics.Typeclasses.tcinstance]
-let impl_2 (v_SIZE: usize) : Core.Convert.t_From (t_MlKemCiphertext v_SIZE) (t_Array u8 v_SIZE) =
-  {
-    f_from_pre = (fun (value: t_Array u8 v_SIZE) -> true);
-    f_from_post = (fun (value: t_Array u8 v_SIZE) (out: t_MlKemCiphertext v_SIZE) -> true);
-    f_from = fun (value: t_Array u8 v_SIZE) -> { f_value = value } <: t_MlKemCiphertext v_SIZE
-  }
+val impl_2 (v_SIZE: usize) : Core.Convert.t_From (t_MlKemCiphertext v_SIZE) (t_Array u8 v_SIZE)
 
 [@@ FStar.Tactics.Typeclasses.tcinstance]
-let impl_3 (v_SIZE: usize) : Core.Convert.t_From (t_MlKemCiphertext v_SIZE) (t_Array u8 v_SIZE) =
-  {
-    f_from_pre = (fun (value: t_Array u8 v_SIZE) -> true);
-    f_from_post = (fun (value: t_Array u8 v_SIZE) (out: t_MlKemCiphertext v_SIZE) -> true);
-    f_from
-    =
-    fun (value: t_Array u8 v_SIZE) ->
-      { f_value = Core.Clone.f_clone #(t_Array u8 v_SIZE) #FStar.Tactics.Typeclasses.solve value }
-      <:
-      t_MlKemCiphertext v_SIZE
-  }
+val impl_3 (v_SIZE: usize) : Core.Convert.t_From (t_MlKemCiphertext v_SIZE) (t_Array u8 v_SIZE)
 
 [@@ FStar.Tactics.Typeclasses.tcinstance]
-let impl_4 (v_SIZE: usize) : Core.Convert.t_From (t_Array u8 v_SIZE) (t_MlKemCiphertext v_SIZE) =
-  {
-    f_from_pre = (fun (value: t_MlKemCiphertext v_SIZE) -> true);
-    f_from_post = (fun (value: t_MlKemCiphertext v_SIZE) (out: t_Array u8 v_SIZE) -> true);
-    f_from = fun (value: t_MlKemCiphertext v_SIZE) -> value.f_value
-  }
+val impl_4 (v_SIZE: usize) : Core.Convert.t_From (t_Array u8 v_SIZE) (t_MlKemCiphertext v_SIZE)
 
 /// A reference to the raw byte slice.
 val impl_6__as_slice (v_SIZE: usize) (self: t_MlKemCiphertext v_SIZE)
@@ -60,33 +40,13 @@ val impl_6__as_slice (v_SIZE: usize) (self: t_MlKemCiphertext v_SIZE)
 type t_MlKemPrivateKey (v_SIZE: usize) = { f_value:t_Array u8 v_SIZE }
 
 [@@ FStar.Tactics.Typeclasses.tcinstance]
-let impl_9 (v_SIZE: usize) : Core.Convert.t_From (t_MlKemPrivateKey v_SIZE) (t_Array u8 v_SIZE) =
-  {
-    f_from_pre = (fun (value: t_Array u8 v_SIZE) -> true);
-    f_from_post = (fun (value: t_Array u8 v_SIZE) (out: t_MlKemPrivateKey v_SIZE) -> true);
-    f_from = fun (value: t_Array u8 v_SIZE) -> { f_value = value } <: t_MlKemPrivateKey v_SIZE
-  }
+val impl_9 (v_SIZE: usize) : Core.Convert.t_From (t_MlKemPrivateKey v_SIZE) (t_Array u8 v_SIZE)
 
 [@@ FStar.Tactics.Typeclasses.tcinstance]
-let impl_10 (v_SIZE: usize) : Core.Convert.t_From (t_MlKemPrivateKey v_SIZE) (t_Array u8 v_SIZE) =
-  {
-    f_from_pre = (fun (value: t_Array u8 v_SIZE) -> true);
-    f_from_post = (fun (value: t_Array u8 v_SIZE) (out: t_MlKemPrivateKey v_SIZE) -> true);
-    f_from
-    =
-    fun (value: t_Array u8 v_SIZE) ->
-      { f_value = Core.Clone.f_clone #(t_Array u8 v_SIZE) #FStar.Tactics.Typeclasses.solve value }
-      <:
-      t_MlKemPrivateKey v_SIZE
-  }
+val impl_10 (v_SIZE: usize) : Core.Convert.t_From (t_MlKemPrivateKey v_SIZE) (t_Array u8 v_SIZE)
 
 [@@ FStar.Tactics.Typeclasses.tcinstance]
-let impl_11 (v_SIZE: usize) : Core.Convert.t_From (t_Array u8 v_SIZE) (t_MlKemPrivateKey v_SIZE) =
-  {
-    f_from_pre = (fun (value: t_MlKemPrivateKey v_SIZE) -> true);
-    f_from_post = (fun (value: t_MlKemPrivateKey v_SIZE) (out: t_Array u8 v_SIZE) -> true);
-    f_from = fun (value: t_MlKemPrivateKey v_SIZE) -> value.f_value
-  }
+val impl_11 (v_SIZE: usize) : Core.Convert.t_From (t_Array u8 v_SIZE) (t_MlKemPrivateKey v_SIZE)
 
 /// A reference to the raw byte slice.
 val impl_13__as_slice (v_SIZE: usize) (self: t_MlKemPrivateKey v_SIZE)
@@ -101,33 +61,13 @@ val impl_13__as_slice (v_SIZE: usize) (self: t_MlKemPrivateKey v_SIZE)
 type t_MlKemPublicKey (v_SIZE: usize) = { f_value:t_Array u8 v_SIZE }
 
 [@@ FStar.Tactics.Typeclasses.tcinstance]
-let impl_16 (v_SIZE: usize) : Core.Convert.t_From (t_MlKemPublicKey v_SIZE) (t_Array u8 v_SIZE) =
-  {
-    f_from_pre = (fun (value: t_Array u8 v_SIZE) -> true);
-    f_from_post = (fun (value: t_Array u8 v_SIZE) (out: t_MlKemPublicKey v_SIZE) -> true);
-    f_from = fun (value: t_Array u8 v_SIZE) -> { f_value = value } <: t_MlKemPublicKey v_SIZE
-  }
+val impl_16 (v_SIZE: usize) : Core.Convert.t_From (t_MlKemPublicKey v_SIZE) (t_Array u8 v_SIZE)
 
 [@@ FStar.Tactics.Typeclasses.tcinstance]
-let impl_17 (v_SIZE: usize) : Core.Convert.t_From (t_MlKemPublicKey v_SIZE) (t_Array u8 v_SIZE) =
-  {
-    f_from_pre = (fun (value: t_Array u8 v_SIZE) -> true);
-    f_from_post = (fun (value: t_Array u8 v_SIZE) (out: t_MlKemPublicKey v_SIZE) -> true);
-    f_from
-    =
-    fun (value: t_Array u8 v_SIZE) ->
-      { f_value = Core.Clone.f_clone #(t_Array u8 v_SIZE) #FStar.Tactics.Typeclasses.solve value }
-      <:
-      t_MlKemPublicKey v_SIZE
-  }
+val impl_17 (v_SIZE: usize) : Core.Convert.t_From (t_MlKemPublicKey v_SIZE) (t_Array u8 v_SIZE)
 
 [@@ FStar.Tactics.Typeclasses.tcinstance]
-let impl_18 (v_SIZE: usize) : Core.Convert.t_From (t_Array u8 v_SIZE) (t_MlKemPublicKey v_SIZE) =
-  {
-    f_from_pre = (fun (value: t_MlKemPublicKey v_SIZE) -> true);
-    f_from_post = (fun (value: t_MlKemPublicKey v_SIZE) (out: t_Array u8 v_SIZE) -> true);
-    f_from = fun (value: t_MlKemPublicKey v_SIZE) -> value.f_value
-  }
+val impl_18 (v_SIZE: usize) : Core.Convert.t_From (t_Array u8 v_SIZE) (t_MlKemPublicKey v_SIZE)
 
 /// A reference to the raw byte slice.
 val impl_20__as_slice (v_SIZE: usize) (self: t_MlKemPublicKey v_SIZE)
@@ -198,61 +138,22 @@ val impl_21__sk
     : Prims.Pure (t_Array u8 v_PRIVATE_KEY_SIZE) Prims.l_True (fun _ -> Prims.l_True)
 
 [@@ FStar.Tactics.Typeclasses.tcinstance]
-let impl (v_SIZE: usize) : Core.Default.t_Default (t_MlKemCiphertext v_SIZE) =
-  {
-    f_default_pre = (fun (_: Prims.unit) -> true);
-    f_default_post = (fun (_: Prims.unit) (out: t_MlKemCiphertext v_SIZE) -> true);
-    f_default
-    =
-    fun (_: Prims.unit) ->
-      { f_value = Rust_primitives.Hax.repeat 0uy v_SIZE } <: t_MlKemCiphertext v_SIZE
-  }
+val impl (v_SIZE: usize) : Core.Default.t_Default (t_MlKemCiphertext v_SIZE)
 
 [@@ FStar.Tactics.Typeclasses.tcinstance]
-let impl_7 (v_SIZE: usize) : Core.Default.t_Default (t_MlKemPrivateKey v_SIZE) =
-  {
-    f_default_pre = (fun (_: Prims.unit) -> true);
-    f_default_post = (fun (_: Prims.unit) (out: t_MlKemPrivateKey v_SIZE) -> true);
-    f_default
-    =
-    fun (_: Prims.unit) ->
-      { f_value = Rust_primitives.Hax.repeat 0uy v_SIZE } <: t_MlKemPrivateKey v_SIZE
-  }
+val impl_7 (v_SIZE: usize) : Core.Default.t_Default (t_MlKemPrivateKey v_SIZE)
 
 [@@ FStar.Tactics.Typeclasses.tcinstance]
-let impl_14 (v_SIZE: usize) : Core.Default.t_Default (t_MlKemPublicKey v_SIZE) =
-  {
-    f_default_pre = (fun (_: Prims.unit) -> true);
-    f_default_post = (fun (_: Prims.unit) (out: t_MlKemPublicKey v_SIZE) -> true);
-    f_default
-    =
-    fun (_: Prims.unit) ->
-      { f_value = Rust_primitives.Hax.repeat 0uy v_SIZE } <: t_MlKemPublicKey v_SIZE
-  }
+val impl_14 (v_SIZE: usize) : Core.Default.t_Default (t_MlKemPublicKey v_SIZE)
 
 [@@ FStar.Tactics.Typeclasses.tcinstance]
-let impl_1 (v_SIZE: usize) : Core.Convert.t_AsRef (t_MlKemCiphertext v_SIZE) (t_Slice u8) =
-  {
-    f_as_ref_pre = (fun (self: t_MlKemCiphertext v_SIZE) -> true);
-    f_as_ref_post = (fun (self: t_MlKemCiphertext v_SIZE) (out: t_Slice u8) -> true);
-    f_as_ref = fun (self: t_MlKemCiphertext v_SIZE) -> self.f_value <: t_Slice u8
-  }
+val impl_1 (v_SIZE: usize) : Core.Convert.t_AsRef (t_MlKemCiphertext v_SIZE) (t_Slice u8)
 
 [@@ FStar.Tactics.Typeclasses.tcinstance]
-let impl_8 (v_SIZE: usize) : Core.Convert.t_AsRef (t_MlKemPrivateKey v_SIZE) (t_Slice u8) =
-  {
-    f_as_ref_pre = (fun (self: t_MlKemPrivateKey v_SIZE) -> true);
-    f_as_ref_post = (fun (self: t_MlKemPrivateKey v_SIZE) (out: t_Slice u8) -> true);
-    f_as_ref = fun (self: t_MlKemPrivateKey v_SIZE) -> self.f_value <: t_Slice u8
-  }
+val impl_8 (v_SIZE: usize) : Core.Convert.t_AsRef (t_MlKemPrivateKey v_SIZE) (t_Slice u8)
 
 [@@ FStar.Tactics.Typeclasses.tcinstance]
-let impl_15 (v_SIZE: usize) : Core.Convert.t_AsRef (t_MlKemPublicKey v_SIZE) (t_Slice u8) =
-  {
-    f_as_ref_pre = (fun (self: t_MlKemPublicKey v_SIZE) -> true);
-    f_as_ref_post = (fun (self: t_MlKemPublicKey v_SIZE) (out: t_Slice u8) -> true);
-    f_as_ref = fun (self: t_MlKemPublicKey v_SIZE) -> self.f_value <: t_Slice u8
-  }
+val impl_15 (v_SIZE: usize) : Core.Convert.t_AsRef (t_MlKemPublicKey v_SIZE) (t_Slice u8)
 
 [@@ FStar.Tactics.Typeclasses.tcinstance]
 let impl_5 (v_SIZE: usize) : Core.Convert.t_TryFrom (t_MlKemCiphertext v_SIZE) (t_Slice u8) =
